theories/ZArith/Pfactor.v
@@ -1,0 +1,763 @@
+Require Import Coq.Program.Wf Relation_Operators Wellfounded.
+Require Import List Sorting. Import ListNotations.
+Require Import Znumtheory ZArith NArith Lia.
+Local Open Scope positive_scope.
+Local Coercion Z.pos : positive >-> Z.
+Local Coercion N.pos : positive >-> N.
+Local Coercion Z.of_N : N >-> Z.
+
+Lemma fst_pair [A B] a b : fst (@pair A B a b) = a. reflexivity. Qed.
+Lemma snd_pair [A B] a b : snd (@pair A B a b) = b. reflexivity. Qed.
+
+Lemma Forall_repeat [A] P x n : P x -> @Forall A P (repeat x n).
+Proof. induction n; cbn [repeat]; auto. Qed.
+
+Lemma repeat_inj [A] (x y : A) n m : repeat x n = repeat y m -> n = m /\ (x = y \/ n = 0%nat).
+Proof.
+  revert y; revert x; revert m; induction n, m; cbn [repeat];
+    inversion 1; intuition eauto; f_equal; eapply IHn; eauto.
+Qed.
+
+Lemma Sorted_repeat [A] R (R_refl : forall x:A, R x x) x n : Sorted R (repeat x n).
+Proof.
+  apply StronglySorted_Sorted.
+  induction n; cbn [repeat]; constructor; auto using Forall_repeat.
+Qed.
+
+Local Hint Constructors StronglySorted : core.
+Lemma StronglySorted_app [A] R (xs ys : list A) :
+  StronglySorted R (xs ++ ys) <->
+  Forall (fun x => Forall (R x) ys) xs /\ StronglySorted R xs /\ StronglySorted R ys.
+Proof.
+  split.
+  { intros H; remember (xs++ys); generalize dependent ys; revert xs; induction H.
+    { intros ? ? []%eq_sym%app_eq_nil; subst; eauto. }
+    intros [|x xs] ys E; cbn [app] in *; subst; eauto.
+    injection E; clear E; intros; subst.
+    specialize (IHStronglySorted xs ys eq_refl) as (?&?&?).
+    rewrite Forall_app in *; intuition eauto. }
+  { apply and_ind; induction 1; apply and_ind; trivial.
+  inversion_clear 1; cbn; constructor; eauto.
+  eapply Forall_app; eauto. }
+Qed.
+
+Lemma NoDup_StronglySorted {A} R xs (R_irrefl : forall x:A, ~R x x)
+  (H : StronglySorted R xs) : NoDup xs.
+Proof.
+  induction H; constructor; trivial.
+  intro; eapply (R_irrefl a), Forall_forall; eauto.
+Qed.
+
+Lemma HdRel_map {A B} (f : A -> B) R x xs :
+  HdRel R (f x) (map f xs) <-> HdRel (fun a b => R (f a) (f b)) x xs.
+Proof.
+  induction xs as [|??[]]; split; inversion_clear 1; cbn [map]; eauto.
+Qed.
+
+Lemma Sorted_map {A B} (f : A -> B) R xs :
+  Sorted R (map f xs) <-> Sorted (fun a b => R (f a) (f b)) xs.
+Proof.
+  induction xs as [|??[]]; split; inversion_clear 1; cbn [map];
+    constructor; try eapply HdRel_map; eauto.
+Qed.
+
+Module Pos.
+  Definition of_N n : positive := match n with N.pos n => n | _ => xH end.
+
+  Definition lt_dec a b : {a<b}+{~a<b}. simple refine (
+    match Pos.compare a b as c return {c = Lt} + {c <> Lt} with
+    | Lt => left eq_refl | _ => right _
+    end); abstract discriminate.
+  Defined.
+  
+  Lemma lt_wf : well_founded Pos.lt.
+  Proof.
+    unshelve eapply Morphisms_Prop.well_founded_morphism.
+    { exact (fun a b => N.lt a b). }
+    { repeat intro; hnf; lia. }
+    { eapply measure_wf with (R:=N.lt), N.lt_wf_0. }
+  Qed.
+
+  Lemma gt_wf c : well_founded (fun a b : positive => b < a <= c).
+  Proof.
+    unshelve eapply Morphisms_Prop.well_founded_morphism.
+    { exact (fun a b => (b < a <= c)%N). }
+    { repeat intro; hnf; lia. }
+    { eapply measure_wf with (R:=(fun a b => (b < a <= c)%N)), N.gt_wf. }
+  Qed.
+
+  Lemma divide_1_r a : (a | 1) <-> a = 1.
+  Proof. split. { inversion_clear 1. nia. } { intros []. exists 1. nia. } Qed.
+
+
+  Definition pow_N p n :=
+    match n with
+    | N0 => xH
+    | Npos q => Pos.pow p q
+    end.
+
+  Lemma Npos_pow_N p n : N.pos (Pos.pow_N p n) = N.pow p n.
+  Proof. cbv [pow_N]; case n; trivial. Qed.
+
+  Definition pow_pred p q := Pos.pow_N p (Pos.pred_N q).
+
+  Lemma Npos_pow_pred p q : N.pos (Pos.pow_pred p q) = N.pow p (Pos.pred_N q).
+  Proof. cbv [pow_pred pow_N]; case Pos.pred_N; trivial. Qed.
+End Pos.
+
+Module N.
+  Local Open Scope N_scope.
+  Definition lt_dec a b : {a<b}+{~a<b}. simple refine (
+    match N.compare a b as c return {c = Lt} + {c <> Lt} with
+    | Lt => left eq_refl | _ => right _
+    end); abstract discriminate.
+  Defined.
+
+  Lemma pos_of_N n : N.pos (Pos.of_N n) = N.max 1 n.
+  Proof. case n; cbn; lia. Qed.
+
+  Lemma pos_of_N_pos n : N.lt 0 n -> N.pos (Pos.of_N n) = n.
+  Proof. case n; cbn; lia. Qed.
+
+  Lemma pos_mul a b : N.pos (a * b) = N.mul a b. Proof. lia. Qed.
+
+  Lemma divide_pos_pos (a b : positive) : N.divide a b <-> Pos.divide a b.
+  Proof.
+    split.
+    { destruct 1 as [x ?]. assert (0 < x)%N by nia. exists (Z.to_pos x). nia. }
+    { destruct 1 as [x ?]. assert (0 < x)%N by nia. exists (Z.to_pos x). nia. }
+  Qed.
+
+  Lemma div_eucl_as_div_mod a b : N.div_eucl a b = (a / b, a mod b).
+  Proof. apply surjective_pairing. Qed.
+
+  Lemma pos_div_eucl_pos_as_div_mod a (b : positive) : N.pos_div_eucl a b = (a / b, a mod b).
+  Proof. rewrite <- div_eucl_as_div_mod; trivial. Qed.
+End N.
+
+Module Z.
+  Lemma pos_of_N n : Z.pos (Pos.of_N n) = Z.max 1 (Z.of_N n).
+  Proof. case n; cbn; lia. Qed.
+
+  Import ZifyClasses.
+  #[global] Instance Op_Pos_of_N : UnOp Pos.of_N.
+  refine ({| TUOp x := Z.max 1 x ; TUOpInj x := _ |}).
+  Proof. exact (pos_of_N x). Defined.
+  Add Zify UnOp Op_Pos_of_N.
+
+  Lemma pos_of_N_pos (n : N) : Z.lt 0 n -> Z.pos (Pos.of_N n) = n.
+  Proof. lia. Qed.
+
+  Lemma divide_pos_pos (a b : positive) : Z.divide a b <-> Pos.divide a b.
+  Proof.
+    split.
+    { destruct 1 as [x ?]. assert (0 < x)%Z by nia. exists (Z.to_pos x). nia. }
+    { destruct 1 as [x ?]. assert (0 < x)%Z by nia. exists (Z.to_pos x). nia. }
+  Qed.
+End Z.
+
+Lemma rel_prime_prime p q (H : p <> q) : prime p -> prime q -> rel_prime p q.
+Proof.
+  intros Hp Hq.
+  apply prime_rel_prime; trivial. intro HX; apply prime_divisors in HX; trivial.
+  pose proof prime_ge_2 _ Hp; pose proof prime_ge_2 _ Hq; lia.
+Qed.
+
+(* ** [val p n] finds largest k s.t. [p^k] divides [n] *)
+
+Local Open Scope N_scope.
+
+Local Definition val_subterm p n (val : forall m, Pos.lt m n -> N) : N :=
+  match N.pos_div_eucl n p with
+  | (N.pos m, 0) => if Pos.lt_dec m n then N.succ (val m ltac:(trivial)) else 0
+  |  _ => 0
+  end.
+Definition val (p : positive) : positive -> N :=
+  Fix (Acc_intro_generator 64 Pos.lt_wf) _ (val_subterm p).
+
+Lemma val_step p n : val p n = ltac:(
+  let y := eval cbv beta delta [val_subterm] in (val_subterm p n (fun y _ => val p y)) in
+  exact y).
+Proof.
+  cbv [val val_subterm].
+  rewrite Init.Wf.Fix_eq; [reflexivity|]; intros.
+  repeat match goal with |- context[match ?x with _ => _ end] => destruct x end;
+    repeat (eapply H || f_equal || trivial).
+Qed.
+
+Lemma val_1_r p : val p 1 = 0.
+Proof. repeat (case p as []; trivial). Qed.
+
+Lemma val_1_l n : val 1 n = 0.
+Proof.
+  rewrite val_step, N.pos_div_eucl_pos_as_div_mod, N.div_1_r, N.mod_1_r.
+  case Pos.lt_dec; lia.
+Qed.
+
+Lemma val_0_iff' (p n : positive) : val p n = 0 <-> (p = xH \/ n mod p <> 0).
+Proof.
+  rewrite val_step, N.pos_div_eucl_pos_as_div_mod.
+  repeat match goal with |- context[match ?x with _ => _ end] => destruct x eqn:? end;
+  zify; Z.to_euclidean_division_equations; nia.
+Qed.
+
+Lemma val_0_iff p n (H : p <> xH) : val p n = 0 <-> n mod p <> 0.
+Proof. rewrite val_0_iff'; lia. Qed.
+
+Lemma val_0_iff_divide p n (H : p <> xH) : val p n = 0 <-> ~ (p | n).
+Proof. rewrite val_0_iff, N.Lcm0.mod_divide; trivial; reflexivity. Qed.
+
+Lemma val_mul p n (H : p <> xH) : val p (Pos.mul p n) = N.succ (val p n).
+Proof.
+  rewrite val_step, N.pos_div_eucl_pos_as_div_mod.
+  rewrite N.pos_mul, N.mul_comm, N.div_mul, N.Div0.mod_mul by lia.
+  case Pos.lt_dec; nia.
+Qed.
+
+Lemma val_mul_pow (p k n : positive) (H : p <> xH) : val p (p ^ k * n) = k + val p n.
+Proof.
+  induction k using Pos.peano_ind;
+    rewrite ?Pos.pow_1_r, ?Pos.pow_succ_r, <-?Pos.mul_assoc, ?val_mul; lia.
+Qed.
+
+Lemma divide_val (p n : positive) : (p ^ val p n | n).
+Proof.
+  induction n using (well_founded_induction Pos.lt_wf); rewrite val_step; cbv [id].
+  assert ((p ^ 0 | n)). { rewrite N.pow_0_r. apply N.divide_1_l. }
+  repeat match goal with |- context[match ?x with _ => _ end] => destruct x eqn:? end; trivial.
+  epose proof N.pos_div_eucl_spec _ _ as E. rewrite Heqp0 in E; subst; rewrite E.
+  rewrite N.pow_succ_r, ?N.add_0_r, N.mul_comm; try eapply N.mul_divide_cancel_r; eauto; lia.
+Qed.
+
+Lemma divide'_val (p n : positive) : ( Pos.of_N (p ^ val p n) | n)%positive.
+Proof.
+  case (divide_val p n) as [q Hq]. exists (Pos.of_N q).
+  enough (q * p ^ val p n = Pos.of_N q * Pos.of_N (p ^ val p n))%N by nia.
+  rewrite ?N.pos_of_N_pos; lia.
+Qed.
+
+Lemma le_val_iff k p n (H : p <> xH) : k <= val p n <-> ( p^k | n ).
+Proof.
+  split.
+  { case (divide_val p n) as [q ->]. exists (q*p^(val p n - k)).
+    rewrite <-N.mul_assoc, <-N.pow_add_r, N.sub_add; trivial. }
+  { inversion 1 as [[|q] ?]; case k as [|k] in *; try lia.
+    assert (n = q * p ^ k)%positive as -> by lia.
+    rewrite Pos.mul_comm, val_mul_pow; try lia. }
+Qed.
+
+Lemma powdivide_as_val (p : positive) k (n : positive) :
+  (p^k | n) <-> (p = xH \/ k <= val p n).
+Proof.
+  case (Pos.eq_dec p xH) as [->|];
+    rewrite ?N.pow_1_l, ?le_val_iff by trivial; intuition apply N.divide_1_l.
+Qed.
+
+Lemma val_iff k p n (H : p <> xH) : val p n = k <-> (p^k|n) /\ ~(p^N.succ k|n).
+Proof. rewrite !powdivide_as_val; lia. Qed.
+
+Lemma divide_as_val (p : positive) (n : positive) :
+  (p | n) <-> (p = xH \/ 1 <= val p n).
+Proof. rewrite <-(N.pow_1_r p). rewrite powdivide_as_val; lia. Qed.
+
+Lemma ndivide_val (p n : positive) (H : p <> xH) k (Hk : val p n < k) : ~ ( p ^ k | n).
+Proof. rewrite <-le_val_iff; try lia. Qed.
+
+Lemma ndivide_val_succ (p n : positive) (H : p <> xH) : ~ ( p * p ^ val p n | n).
+Proof. rewrite <-N.pow_succ_r, <-le_val_iff; try lia. Qed.
+
+Lemma ndivide_val_div (p n : positive) (H : p <> xH) : ~ ( p | n / p ^ val p n ).
+Proof.
+  intros [x X]; case (divide_val p n) as [q Hq].
+  rewrite Hq, N.div_mul in X by lia; rewrite X in Hq.
+  eapply (ndivide_val_succ p n); trivial; exists x; lia.
+Qed.
+
+(** * Factorization into prime powers *)
+
+Local Open Scope positive_scope.
+
+Definition ppfactor_lt := MR Pos.lt (uncurry Pos.sub).
+
+Lemma ppfactor_wf : well_founded ppfactor_lt.
+Proof. apply measure_wf, Pos.lt_wf. Qed.
+
+Definition ppfactor_subterm (n_i : positive * positive) (ppfactor : forall m_j, ppfactor_lt m_j n_i -> list (positive * positive))
+  : list (positive * positive).
+Proof.
+simple refine (
+  let n := fst n_i in let i := Pos.succ (snd n_i) in
+  if Pos.lt_dec n (i*i) then if Pos.eqb 1 n then [] else [(n, 1)] else
+  let k := val i n in
+  let j := if N.odd i then Pos.succ i else i in
+  if N.eq_dec 0 k    then ppfactor (n, j) _
+  else (i, Pos.of_N k) :: ppfactor (Pos.of_N (n/i^k), j) _);
+clear ppfactor; abstract (
+ cbv [ppfactor_lt MR uncurry]; subst n; destruct n_i as [n i']; cbn [fst snd] in *; try solve
+ [ subst i; case N.odd in *; lia
+ | case (divide'_val i n) as [q Eq]; case N.odd in *; zify; Z.div_mod_to_equations; nia]).
+Defined.
+
+Definition ppfactor_rec : positive * positive -> list (positive * positive) :=
+  Fix (Acc_intro_generator 64 ppfactor_wf) _ ppfactor_subterm.
+
+Lemma ppfactor_rec_step p : ppfactor_rec p = ltac:(
+  let y := eval cbv beta delta [ppfactor_subterm] in (ppfactor_subterm p (fun y _ => ppfactor_rec y)) in
+  exact y).
+Proof.
+  cbv [ppfactor_rec ppfactor_subterm].
+  rewrite Init.Wf.Fix_eq; [reflexivity|]; intros.
+  repeat match goal with |- context[match ?x with _ => _ end] => destruct x end;
+    repeat (eapply H || f_equal || trivial).
+Defined.
+
+Definition ppfactor p := ppfactor_rec (p, 1).
+
+(*
+Compute ppfactor 24.
+Compute ppfactor 1311.
+Compute ppfactor (2^16-1).
+Compute ppfactor (2^16+1).
+Time Compute ppfactor (2^32-1). (* 0.003s *)
+Time Compute ppfactor (2^32+1). (* 0.02s *)
+Time Compute ppfactor (2^31+1). (* 0.3s *)
+Time Compute ppfactor (2^31-1). (* 0.6s *)
+Time Compute ppfactor (2^46-1). (* 3.2s *)
+*)
+
+Lemma fold_right_nil [A B] (f : B -> A -> A) a : fold_right f a nil = a.
+Proof. reflexivity. Qed.
+
+Lemma fold_right_cons [A B] (f : B -> A -> A) a x xs :
+  fold_right f a (x::xs) = f x (fold_right f a xs). Proof. reflexivity. Qed.
+
+Local Notation Π := (fold_right Pos.mul 1).
+
+Lemma prod_app ps qs : Π (ps ++ qs) = Π ps * Π qs.
+Proof. induction ps; cbn [fold_right app]; rewrite ?IHps, ?Pos.mul_assoc, ?Pos.mul_1_l; trivial. Qed.
+
+Lemma prod_concat ps : Π (concat ps) = Π (map Π ps).
+Proof. induction ps; cbn [fold_right concat map]; rewrite ?prod_app; congruence. Qed.
+
+Lemma prod_repeat q c : Π (repeat q (Pos.to_nat c)) = q ^ c.
+Proof.
+  induction c using Pos.peano_ind; trivial.
+  rewrite ?Pos2Nat.inj_succ, ?Pos.pow_succ_r; cbn [repeat fold_right]; congruence.
+Qed.
+
+Lemma divide_in_prod ps : Forall (fun p => (p | Π ps)) ps.
+Proof.
+  induction ps; cbn [fold_right concat map]; constructor; trivial.
+  { apply Pos.divide_mul_l. exists 1. lia. }
+  { eapply Forall_impl; eauto; cbv beta; intros q [y ->]; exists (a*y); lia. }
+Qed.
+
+Lemma prod_ppfactor_rec p i : Π (map (uncurry Pos.pow) (ppfactor_rec (p, i))) = p.
+Proof.
+  change p with (fst (p, i)) at 2;
+  induction (p, i) as [[p' i']IH] using (well_founded_induction ppfactor_wf);
+    clear i p; rename p' into p; rewrite ppfactor_rec_step; cbn [fst snd].
+  set (Pos.succ i') as i.
+  set (if N.odd _ then _ else _) as j; assert (i' < j) by (case N.odd in *; subst i; lia).
+  repeat match goal with |- context[match ?x with _ => _ end] => destruct x eqn:? end;
+  repeat (cbn [uncurry (* map -- Qed timeout *)]; rewrite ?fold_right_nil, ?fold_right_cons, ?map_cons);
+    rewrite ?IH; cbn [fst snd];
+    try rapply ppfactor_subterm_subproof; try rapply ppfactor_subterm_subproof0; trivial;
+    try apply Pos.eqb_eq in Heqb; try lia.
+  case (divide_val i p) as [q Hq].
+  rewrite Hq, N.div_mul, Pos.mul_comm by lia.
+  enough (Pos.of_N q * i ^ Pos.of_N (val i p) = p)%N by lia;
+    rewrite ?N.pos_of_N_pos; lia.
+Qed.
+
+Lemma prod_ppfactor p : Π (map (uncurry Pos.pow) (ppfactor p)) = p.
+Proof. apply prod_ppfactor_rec. Qed.
+
+Lemma Private_ppfactor_rec_correct
+  (n i : positive) (ps := map fst (ppfactor_rec (n, i))) :
+  (forall d, 1 < d -> (d | fst (n, i)) -> Pos.succ (snd (n, i)) <= d)%Z ->
+  StronglySorted Pos.lt ps /\ Forall (fun p => prime (Z.pos p) /\ ( snd (n, i) < p <= fst (n, i))) ps.
+Proof.
+  induction (n, i) as [[n' i']IH] using (well_founded_induction ppfactor_wf);
+    clear n i; rename n' into n; subst ps; rewrite ppfactor_rec_step; cbn [fst snd].
+  intros I; case Pos.lt_dec as []. (* base case *)
+  { case (Pos.eqb_spec 1 n) as []; repeat split; cbn [map fst];
+      intuition eauto using SSorted_cons, SSorted_nil;
+      try apply Forall_cons; try apply Forall_nil; split.
+    { apply prime_alt; split; [lia|]; intros a?[b ?].
+      pose proof I a ltac:(lia) ltac:(exists b; lia).
+      pose proof I b ltac:(nia) ltac:(exists a; lia). nia. }
+    { pose proof (I n ltac:(lia) ltac:(reflexivity)); lia. } }
+  set (Pos.succ i') as i in *. (* bound variables *)
+  set (if N.odd _ then _ else _) as j';
+    assert (j' = i'+1 \/ j'=i'+2) by (case N.odd in *; subst i; lia).
+  case (divide'_val i n) as [q Hq].
+  set (val i n) as k in *.
+  assert (q = Pos.of_N (n / i ^ k)). { zify; Z.div_mod_to_equations; nia. }
+  assert (forall d, (1 < d)%Z -> (d | n) -> d <> i -> (Pos.succ j' <= d))%Z as I_.
+  { intros a ? [b ab] ?. pose proof (I a ltac:(lia) ltac:(exists b; trivial)).
+    case N.odd eqn:E; [|lia]. rewrite <-N.even_succ, N.even_spec in E.
+    case E as [j]. enough (a <> Pos.succ i) by lia; intro.
+    unshelve epose proof (I 2 _ ltac:(exists (b*j)%Z)); lia. }
+  case N.eq_dec as []; rewrite ?map_cons.
+  { case (IH (n, j') ltac:(try rapply ppfactor_subterm_subproof; trivial)) as (A&B);
+      clear IH; cbn [fst snd] in *. (* recursive case withot division *)
+    { intros; apply I_; trivial. (* invariant preserved: i wasn't a ppfactor *)
+      intros ->; case (proj1 (val_0_iff_divide i n ltac:(lia)) ltac:(lia)).
+      case H2 as [b ?];  exists (Z.to_N b); lia. }
+    eapply conj, Forall_impl; eauto; intuition lia. }
+  (* recursive case with division *) eassert (I' : _); try
+    case (IH (Pos.of_N (n / i ^ k), j') ltac:(rapply ppfactor_subterm_subproof0; trivial) I') as (A&B);
+      clear IH; rewrite ?fst_pair, ?snd_pair in * (* cbn -> Qed timeout *).
+  { (* invariant restored: i is no longer a facter  *)
+    intros ? ? Hb; apply I_; trivial; case Hb as [b]. { exists (b*i^k)%Z; nia. }
+    intros->. subst k. apply (ndivide_val_succ i n); [|exists (Z.to_N b)];nia. }
+  eassert (O : _ ); [|split; constructor; [trivial|exact O|split;[|nia]| ] ].
+  { (* range of recursive ppfactors *) epose proof divide_in_prod _ as D;
+    erewrite (prod_ppfactor_rec (Pos.of_N (n / i ^ k)) j'), Forall_map in D.
+    eapply Forall_map in B. epose proof Forall_and B D as F; cbv beta in *.
+    eapply Forall_map, Forall_impl, F; clear A D F; intros [f e] ([]&x&Hx);
+      cbv [fst snd uncurry] in *.
+    unshelve epose proof I f _ _; try nia.
+    exists (Pos.of_N (i ^ k)*x*(f^Pos.pred_N e))%N.
+    enough (f^e = f * f ^ Pos.pred_N e)%N by nia.
+    replace (N.pos e) with (N.succ (N.pred e)) by lia.
+    rewrite N.pow_succ_r'; f_equal; lia. }
+  { (* found a ppfactor *) apply prime_alt; split; try lia.
+    intros a ? [b]. unshelve epose proof I a _ ltac:(exists (q*a^(k-1)*b^k)%Z); try nia.
+    enough (i ^ k = (a * a ^ (k - 1)) * b ^ k :> Z)%Z by lia.
+    rewrite <-Z.pow_succ_r, Z.sub_1_r, Z.succ_pred, <-Z.pow_mul_l by lia; f_equal; lia. }
+  { eapply Forall_impl, B; intuition nia. }
+Qed.
+
+Lemma Sorted_ppfactor n : Sorted Pos.lt (map fst (ppfactor n)).
+Proof. eapply StronglySorted_Sorted, Private_ppfactor_rec_correct; cbn [fst snd]; lia. Qed.
+
+Lemma NoDup_ppfactor n : NoDup (ppfactor n).
+Proof.
+  eapply NoDup_StronglySorted with (R:=fun a b=>fst a<fst b),
+    Sorted_StronglySorted, Sorted_map, Sorted_ppfactor ; repeat intro; try lia.
+Qed.
+
+Local Notation prime := (fun p => prime (Z.pos p)).
+
+Lemma fst_ppfactor n : Forall (fun p => prime p /\ 2 <= p <= n) (map fst (ppfactor n)).
+Proof. eapply Forall_impl, Private_ppfactor_rec_correct; cbn [fst snd]; intuition lia. Qed.
+
+Lemma prime_ppfactor n : Forall prime (map fst (ppfactor n)).
+Proof. eapply Forall_impl, fst_ppfactor; cbv beta; intuition idtac. Qed.
+
+Lemma range_ppfactor n : Forall (fun p => 2 <= p <= n) (map fst (ppfactor n)).
+Proof. eapply Forall_impl, fst_ppfactor; cbv beta; intuition idtac. Qed.
+
+Lemma ppfactor_inj a b (H : ppfactor a = ppfactor b) : a = b.
+Proof. rewrite <-(prod_ppfactor a), <-(prod_ppfactor b); congruence. Qed.
+
+(** * Factorization into primes *)
+
+Local Notation expand := (flat_map (fun '(p, k) => repeat p (Pos.to_nat k))).
+Definition factor n := expand (ppfactor n).
+
+Local Lemma prod_expand xs : Π (expand xs) = Π (map (uncurry Pos.pow) xs).
+Proof.
+  erewrite flat_map_concat_map, prod_concat, map_map, map_ext; trivial.
+  intros []; apply prod_repeat.
+Qed.
+
+Lemma prod_factor n : Π (factor n) = n.
+Proof. rewrite <-prod_ppfactor, <-prod_expand; trivial. Qed.
+
+Local Lemma Forall_expand [A] (P : A -> Prop) xs :
+  Forall P (expand xs) <-> Forall P (map fst xs).
+Proof.
+  rewrite flat_map_concat_map, Forall_concat, !Forall_map, !Forall_forall.
+  split; intros H [] I; specialize (H _ I); cbn [fst] in *;
+    eauto using Forall_repeat.
+  destruct repeat eqn:? in H.
+  { apply (f_equal (@length _)) in Heql; rewrite repeat_length in Heql;
+     cbn [length] in Heql; lia. }
+  eapply repeat_eq_cons in Heql; intuition subst. inversion_clear H; trivial.
+Qed.
+
+Lemma prime_factor n : Forall prime (factor n).
+Proof. eapply Forall_expand, Forall_impl, prime_ppfactor; eauto. Qed.
+
+Lemma range_factor n : Forall (fun p => 2 <= p <= n) (factor n).
+Proof. eapply Forall_expand, Forall_impl, range_ppfactor; eauto. Qed.
+
+Lemma Sorted_factor n : Sorted Pos.le (factor n).
+Proof.
+  pose proof Sorted_ppfactor n as H.
+  eapply Sorted_StronglySorted in H; try rapply Pos.lt_trans.
+  cbv [factor]; set (ppfactor n) as pps in *; clearbody pps.
+  induction pps as [|[p k]]; cbn [repeat flat_map]; trivial.
+  inversion_clear H as [| x y Hsort Hlt  ].
+  eapply StronglySorted_Sorted, StronglySorted_app; repeat split;
+    try eapply Sorted_StronglySorted; try rapply Pos.le_trans;
+    eauto using Sorted_repeat, Pos.le_refl.
+  eapply Forall_forall; intros ? ->%repeat_spec.
+  eapply Forall_forall; intros q [[] [H ->%repeat_spec]]%in_flat_map.
+  eapply Forall_forall in Hlt; [|eapply in_map, H]; eauto using Pos.lt_le_incl.
+Qed.
+
+Lemma factor_inj a b (H : factor a = factor b) : a = b.
+Proof. rewrite <-(prod_factor a), <-(prod_factor b); congruence. Qed.
+
+(** Euler's totient function *)
+
+Definition totientpp p e := Pos.pow_pred p e * Pos.pred p.
+Definition totient n := Π (map (uncurry totientpp) (ppfactor n)).
+
+(*
+Compute totient 1.
+Compute totient 9.
+Compute totient 20.
+Compute totient 80.
+Compute totient 90.
+Compute totient 352.
+Time Compute totient (2^46-1).
+*)
+
+(** * Fundamental theorem of arithmetic *)
+
+Require Import Permutation.
+
+Lemma fold_right_Permutation {A} (f:A->A->A) (H : forall x y z, f x (f y z) = f y (f x z)) xs ys : Permutation xs ys -> forall o, fold_right f o xs = fold_right f o ys.
+Proof. induction 1; cbn [fold_right]; intuition try congruence. Qed.
+
+Lemma StronglySorted_Permutation_unique {A} (R : A->A->Prop)
+  (R_asym : forall x y, R x y -> R y x -> x = y) xs ys
+  : StronglySorted R xs -> StronglySorted R ys -> Permutation xs ys -> xs = ys.
+Proof.
+  intros H; revert ys; induction H as [|x xs Hxs IH].
+  {  intros ? ? ?%Permutation_nil; congruence. }
+  intros [|y ys].
+  { intros ? ?%Permutation_sym%Permutation_nil; congruence. }
+  inversion_clear 1; intros.
+  enough (x = y) as <- by (f_equal; eauto using Permutation_cons_inv); clear IH.
+  assert (Forall (fun v => x = v \/ R x v) (y::ys)) as E. {
+    eapply Permutation_Forall; try eassumption.
+    constructor. left. trivial. eauto using Forall_impl. }
+  inversion_clear E as []; intuition try congruence.
+  assert (Forall (fun v => y = v \/ R y v) (x::xs)) as E. {
+    eapply Permutation_Forall; try symmetry; try eassumption.
+    constructor. left. trivial. eauto using Forall_impl. }
+  inversion_clear E; intuition try congruence; eauto.
+Qed.
+
+Lemma Sorted_Permutation_unique {A} (R : A->A->Prop)
+  (R_trans : Relations_1.Transitive R) (R_asym : forall x y, R x y -> R y x -> x = y)
+  xs ys : Sorted R xs -> Sorted R ys -> Permutation xs ys -> xs = ys.
+Proof.
+  intros. eapply StronglySorted_Permutation_unique;
+    eauto using Sorted_StronglySorted.
+Qed.
+
+Lemma prime_product_1 ps : Forall prime ps -> Π ps = 1 -> ps = nil.
+Proof.
+  destruct 1; cbn; intuition idtac.
+  eapply prime_ge_2 in H.
+  nia.
+Qed.
+
+Lemma prime_divisor_of_prime_product :
+  forall p qs, prime p -> Forall prime qs -> (p | Π qs)%Z -> In p qs.
+Proof.
+  induction 2 as [|q qs]; cbn [fold_right]; intros.
+  { apply prime_ge_2 in H; apply Z.divide_1_r_abs in H0; lia. }
+  case (Pos.eq_dec p q); (intuition (subst; eauto using in_eq)); []; right.
+  pose proof rel_prime_prime p q ltac:(lia) ltac:(trivial) ltac:(trivial).
+  apply Zgcd_1_rel_prime in H3. rewrite Pos2Z.inj_mul in *. eauto using Z.gauss.
+Qed.
+
+Lemma prime_divisor_of_prime_power_product q pps (Hq : prime q)
+  (Hp : Forall prime (map fst pps)) (Hd : (q | Π (map (uncurry Pos.pow) pps))%Z)
+  : In q (map fst pps).
+Proof.
+  unshelve epose proof prime_divisor_of_prime_product q (expand pps) _ _ _ as H;
+    rewrite ?prod_expand; try apply Forall_expand; trivial.
+  rewrite in_flat_map in H; case H as ([p k]&?&->%repeat_spec).
+  apply in_map_iff; exists (p, k); eauto.
+Qed.
+
+Lemma fundamental_theorem_of_arithmetic_Permutation' ps :
+  Forall prime ps -> forall qs, Forall prime qs -> Π ps = Π qs -> Permutation ps qs.
+Proof.
+  induction 1 as [|p ps]; cbn [fold_right]; intros.
+  { eapply prime_product_1 in H; subst; trivial; lia. }
+  epose proof prime_divisor_of_prime_product p qs ltac:(trivial) ltac:(trivial) ltac:(exists(Π ps);lia).
+  eapply in_split in H3; case H3 as (qs0&qs1&?); subst qs.
+  eapply perm_trans, Permutation_middle; try apply perm_skip, IHForall.
+  { eapply Permutation_Forall in H1; try (symmetry; eapply Permutation_middle);
+     inversion_clear H1; trivial. }
+  { pose proof prime_ge_2 _ H.
+    symmetry in H2; erewrite fold_right_Permutation in H2;
+      try (symmetry; eapply Permutation_middle); cbn [fold_right] in *; nia. }
+Qed.
+
+Lemma fundamental_theorem_of_arithmetic_Permutation (a : positive) ps :
+  Forall prime ps -> Π ps = a -> Permutation ps (factor a).
+Proof.
+  intros;eapply fundamental_theorem_of_arithmetic_Permutation';
+    rewrite ?prod_factor; eauto using prime_factor.
+Qed.
+
+Lemma fundamental_theorem_of_arithmetic (a : positive) ps :
+  Sorted Pos.le ps -> Forall prime ps -> Π ps = a -> ps = factor a.
+Proof.
+  intros; eapply (Sorted_Permutation_unique Pos.le);
+    try eapply fundamental_theorem_of_arithmetic_Permutation;
+    eauto using Sorted_factor; cbv [Relations_1.Transitive]; lia.
+Qed.
+
+Lemma factor_complete p n : prime p -> (p | n) -> In p (factor n).
+Proof.
+  intros Hp [n' Hq].
+  unshelve epose proof fundamental_theorem_of_arithmetic_Permutation n (p::factor n') _ _;
+    rewrite ?fold_right_cons, ?prod_factor; auto using prime_factor; try lia.
+  eauto using Permutation_in, in_eq.
+Qed.
+
+Lemma factor_prime p (H : prime p) : factor p = [p].
+Proof.
+  symmetry; eapply fundamental_theorem_of_arithmetic;
+    auto; apply Pos.mul_1_r.
+Qed.
+
+Lemma factor_prime_power p (H : prime p) k :
+  factor (p^k) = repeat p (Pos.to_nat k).
+Proof.
+  symmetry; eapply fundamental_theorem_of_arithmetic;
+    auto using Sorted_repeat, Forall_repeat, Pos.le_refl, prod_repeat.
+Qed.
+
+Lemma NoDup_ppfactor' n : NoDup (map (uncurry Pos.pow) (ppfactor n)).
+Proof.
+  eapply FinFun.Injective_map_NoDup_in, NoDup_ppfactor.
+  intros [p e] [q k]; cbn [uncurry]; intros A B E.
+  eapply Forall_forall in A; try eapply Forall_map, prime_ppfactor.
+  eapply Forall_forall in B; try eapply Forall_map, prime_ppfactor.
+  eapply (f_equal factor) in E; rewrite 2factor_prime_power in E by trivial.
+  eapply repeat_inj in E; intuition subst; f_equal; lia.
+Qed.
+
+Lemma factor_mul_Permutation a b : Permutation (factor (a*b)) (factor a ++ factor b).
+Proof.
+  rewrite <-(prod_factor a) at 1; rewrite <-(prod_factor b) at 1;
+  specialize (prime_factor b); specialize (prime_factor a).
+  intros. symmetry. eapply fundamental_theorem_of_arithmetic_Permutation.
+  { eapply Forall_app; eauto. } { rewrite ?prod_app, ?prod_factor; trivial. }
+Qed.
+
+Lemma divide_factor n : Forall (fun d => (d | n)) (factor n).
+Proof.
+  rewrite <-(prod_factor n); rewrite prod_factor at 1.
+    generalize (factor n) as xs; induction xs;
+    rewrite ?fold_right_nil, ?fold_right_cons; constructor.
+  { exists (Π xs). lia. }
+  { eapply Forall_impl, IHxs; intros x [y ?]; exists (a*y); lia. }
+Qed.
+
+Lemma in_factor p n : In p (factor n) <-> prime p /\ (p | n).
+Proof.
+  pose proof proj1 (Forall_forall _ _) (prime_factor n).
+  pose proof proj1 (Forall_forall _ _) (divide_factor n).
+  intuition auto using factor_complete.
+Qed.
+
+Lemma disjoint_factor_coprime (a b : positive) (H : Pos.gcd a b = 1)
+  p (Ha : In p (factor a)) (Hb : In p (factor b)) : False.
+Proof.
+  apply (f_equal Z.pos) in H; rewrite Pos2Z.inj_gcd in H.
+  pose proof (proj1 (Forall_forall _ _) (range_factor _)) _ Ha; cbv beta in *.
+  apply (proj1 (Forall_forall _ _) (divide_factor _)), Z.divide_Zpos in Ha.
+  apply (proj1 (Forall_forall _ _) (divide_factor _)), Z.divide_Zpos in Hb.
+  apply Zgcd_1_rel_prime in H; inversion H as [_ _ H']; specialize (H' p Ha Hb).
+  apply Z.divide_1_r in H'; lia.
+Qed.
+
+Local Opaque Z.gcd.
+
+Lemma factor_ind (P : positive -> Prop)
+  (init : P 1)
+  (step : forall n p, P n -> prime p ->
+    (forall q, prime q -> Z.divide q n -> q <= p) -> P (n * p))
+  : forall n, P n.
+Proof.
+  intros n; revert step; revert init.
+  rewrite <-(prod_factor n).
+  specialize (Sorted_factor n); cbv zeta.
+  specialize (prime_factor n); cbv zeta.
+  specialize (range_factor n); cbv zeta.
+  set (factor n) as ps; clearbody ps.
+  induction ps as [|p ps] using rev_ind; cbn; trivial.
+  rewrite prod_app; cbn [map fold_right]; rewrite Pos.mul_1_r.
+  intros [A H']%Forall_app [B H]%Forall_app C ? ?; inversion_clear H.
+  eapply Sorted_StronglySorted in C; try exact Pos.le_trans.
+  eapply StronglySorted_app in C; case C as (?&C&?).
+  eapply step; eauto; try eapply IHps; eauto using StronglySorted_Sorted.
+  intros q ? ?%prime_divisor_of_prime_product; eauto.
+  eapply Forall_forall in H; eauto. inversion_clear H; eauto.
+Qed.
+
+Lemma ppfactor_ind (P : positive -> Prop)
+  (init : P 1)
+  (step : forall n p k, P n -> prime p -> Z.gcd n p = xH ->
+    (forall q, prime q -> Z.divide q n -> q < p) -> P (n * p ^ k))
+  : forall n, P n.
+Proof.
+  intros n; revert step; revert init.
+  rewrite <-(prod_ppfactor n).
+  specialize (Sorted_ppfactor n); cbv zeta.
+  specialize (prime_ppfactor n); cbv zeta.
+  specialize (range_ppfactor n); cbv zeta.
+  set (ppfactor n) as pps; clearbody pps.
+  induction pps as [|[p k]] using rev_ind; cbn; trivial.
+  rewrite map_app, map_cons; cbn [map].
+  rewrite map_app, map_cons, prod_app; cbn [map fold_right uncurry].
+  rewrite Pos.mul_1_r.
+  intros H H0 H1 **.
+  eapply Forall_app in H; case H as [? [[] _]%Forall_cons_iff]; cbn [fst snd] in *.
+  eapply Forall_app in H0; case H0 as [? [? _]%Forall_cons_iff]; cbn [fst snd] in *.
+  eapply Sorted_StronglySorted in H1; try exact Pos.lt_trans.
+  eapply StronglySorted_app in H1; case H1 as (?&?&?).
+  eapply step; eauto using Forall_app.
+  eapply IHpps; eauto using Forall_app;
+    try split; eauto using StronglySorted_Sorted.
+  { eapply Zgcd_1_rel_prime, rel_prime_sym, prime_rel_prime; trivial.
+    intros X%prime_divisor_of_prime_power_product; trivial.
+    eapply Forall_forall in H1; eauto; inversion H1; lia. }
+  { intros q Hq Hd%prime_divisor_of_prime_power_product; trivial.
+    eapply Forall_forall in H1; eauto; inversion H1; trivial. }
+Qed.
+
+Lemma in_ppfactor p k n : In (p, k) (ppfactor n) <-> (prime p /\ val p n = k).
+Proof.
+  rewrite <-(prod_ppfactor n) at 2.
+  induction (ppfactor n); cbn [In]; rewrite ?IHl, ?map_cons, ?fold_right_cons.
+  { rewrite val_1_r. intuition try lia. }
+  epose proof val_0_iff_divide p (Π (map (uncurry Pos.pow) l)) _.
+  split; [intros []|intros ?]; subst; cbn [uncurry].
+  { rewrite val_mul_pow by admit.
+    rewrite (proj2 H); try lia.
+    epose proof prime_divisor_of_prime_power_product p l _ _.
+    all : admit. }
+  admit.
+  case H as [].
+  destruct (val p (Π (map (uncurry Pos.pow) l))) eqn:?; [left|right].
+  { specialize (H eq_refl). rewrite val_0_iff_divide in Heqn0 by admit.
+    case Heqn0.
+Admitted.
+
+Lemma val_ext a b : (forall p, prime p -> val p a = val p b) -> a = b.
+Proof.
+  intros H.
+  rewrite <-(prod_ppfactor a) at 1; rewrite <-(prod_ppfactor b) at 1.
+  eapply fold_right_Permutation, NoDup_Permutation;
+    try apply NoDup_ppfactor'; try lia; intros.
+  rewrite !in_map_iff.
+  split; intros [[q k] [? []%in_ppfactor]];
+    exists (q, k); split; trivial;
+    apply in_ppfactor; split; trivial;
+    rewrite H||rewrite<-H; trivial.
+Qed.
